theories/Itauto.v
@@ -21,17 +21,37 @@ Ltac gen_conflicts tac :=
 Ltac vitautog :=
   (* Reify the conclusion *)
   cdcl_change;
-  let n := fresh in
-  (intro n ;
+  let n := fresh "n" in
+  let m := fresh "m" in
+  let f := fresh "f" in
+  (intros n m f ;
   (* Apply soundness proof and compute *)
   apply (hcons_bprover_correct (KeyInt.nat_of_int n));
   vm_compute; reflexivity).
 
+(*Ltac vitautog :=
+  (* Reify the conclusion *)
+  cdcl_change;
+  let n := fresh "n" in
+  let mb := fresh "mb" in
+  let md := fresh "md" in
+  let m := fresh "m" in
+  let f := fresh "f" in
+  (intros n mb md m f;
+  (* Apply soundness proof and compute *)
+   apply (hcons_tauto_prover_correct m md mb (KeyInt.nat_of_int n));
+   [reflexivity | reflexivity | vm_compute; reflexivity]).
+*)
+
+
 (** [nitautog] same as [vitauto] but uses native_compute *)
 Ltac nitautog :=
+  (* Reify the conclusion *)
   cdcl_change;
-  let n := fresh in
-  (intro n ;
+  let n := fresh "n" in
+  let m := fresh "m" in
+  let f := fresh "f" in
+  (intros n m f ;
   (* Apply soundness proof and compute *)
   apply (hcons_bprover_correct (KeyInt.nat_of_int n));
   native_compute; reflexivity).
@@ -41,15 +61,10 @@ Ltac vitauto :=
   cdcl_generalize ;
   vitautog.
 
-Ltac itauto_use_tauto := constr:(false).
-
 Ltac itauto tac  :=
   gen_conflicts tac ;
-  clear;
-  lazymatch itauto_use_tauto with
-  | true => tauto
-  | false => vitautog
-  end.
+  vitautog.
+
 
 Ltac itautor tac := let t := solve[tac | itauto tac] in itauto t.
 
